theories/FOL/Reductions/PCPb_to_FOL_class.v
@@ -1,9 +1,13 @@
 (* * Classical Natural Deduction *)
 
 
-From Undecidability.FOL Require Export PCPb_to_FOL.
-Require Import Undecidability.PCP.Reductions.PCPb_iff_dPCPb.
+From Undecidability.FOL Require Import FOL Reductions.PCPb_to_FOL Util.Syntax_facts Util.Deduction Util.Tarski.
+Require Import Undecidability.PCP.Reductions.PCPb_iff_dPCPb Undecidability.PCP.PCP.
 From Undecidability.Synthetic Require Import Definitions DecidabilityFacts EnumerabilityFacts ReducibilityFacts.
+Require Import List.
+Require Import Undecidability.Shared.ListAutomation.
+Import ListNotations.
+
 (* ** Double Negation Translation *)
 
 Implicit Type b : falsity_flag.
@@ -19,7 +23,7 @@ Proof.
   - exact P.
 Defined.
 
-Hint Constructors prv : core.
+Local Hint Constructors prv : core.
 
 Fixpoint cast {b} (phi : form b) : form falsity_on :=
   match phi with
@@ -125,7 +129,7 @@ Proof.
     + apply IHphi.
     + apply II. eapply IE. { apply Ctx. right. left. cbn. reflexivity. }
       apply II. eapply IE. { apply Ctx. right. left. reflexivity. }
-      replace (trans phi[up sigma]) with ((subst_form (up ↑) (trans (subst_form (up sigma) phi)))[($0)..]).
+      replace (trans phi[up sigma]) with (((trans (phi[up sigma]))[up ↑])[($0)..]) at 4.
       * apply AllE. apply Ctx. now left.
       * setoid_rewrite trans_subst. cbn. repeat setoid_rewrite subst_comp.
         apply subst_ext. intros n. unfold funcomp. cbn.
